theories/L6_PCPS/rel_comp.v
@@ -3,38 +3,63 @@ Require Import Coq.NArith.BinNat Coq.Relations.Relations Coq.MSets.MSets Coq.MSe
         Coq.Lists.List Coq.omega.Omega Coq.Sets.Ensembles.
 Require Import L6.cps L6.eval L6.cps_util L6.identifiers L6.ctx L6.set_util
         L6.Ensembles_util L6.List_util L6.size_cps L6.tactics L6.relations. 
-Require Export L6.logical_relations L6.logical_relations_cc.
+Require Export L6.logical_relations L6.logical_relations_cc L6.alpha_conv L6.inline_letapp.
 Require Import compcert.lib.Coqlib.
 
 Import ListNotations.
 
 Close Scope Z_scope.
 
-Section RelComp.
+Section Compose.
 
-
-  Context (cenv : ctor_env) (ctag : ctor_tag).
-
-  Definition rel {A} := PostT -> PostGT -> A -> A -> Prop.
+  Context {A : Type}.
   
-  Inductive R_n {A} (R : PostT -> PostGT -> A -> A -> Prop) : nat -> PostT -> PostGT -> A -> A -> Prop :=
+  Definition post_property := A -> A -> PostT -> PostGT -> Prop.
+  
+  Context (well_formed : A -> Prop)
+          (post_prop : post_property).
+  
+  
+  Definition wf_pres (e1 e2 : A) := well_formed e1 -> well_formed e2. 
+  
+  Definition rel := PostT -> PostGT -> A -> A -> Prop.
+  
+  Inductive R_n (R : PostT -> PostGT -> A -> A -> Prop) : nat -> PostT -> PostGT -> A -> A -> Prop :=
   | One :
       forall (P : PostT) (PG : PostGT) (c1 : A) (c2: A),
         R P PG c1 c2 ->
+        wf_pres c1 c2 ->        
         R_n R 0%nat P PG c1 c2
   | More :
       forall (n : nat) (P : PostT) (PG : PostGT) (c1 : A) (c2: A) P1 P2 PG1 PG2 c',
         R P1 PG1 c1 c' ->
         R_n R n P2 PG2 c' c2 ->
+        wf_pres c1 c2 ->
+        post_prop c1 c2 P PG ->
         same_relation _ (compose P1 P2) P ->
         same_relation _ (compose PG1 PG2) PG ->
         R_n R (S n) P PG c1 c2.
-    
-  Definition preord_exp_n n := R_n (fun P PG c1 c2 => forall k, preord_exp cenv P PG k c1 c2) n.  
 
-  Definition preord_val_n n := R_n (fun P PG c1 c2 => forall k, preord_val cenv PG k c1 c2) n.
+End Compose.
 
-  Definition preord_res_n n := R_n (fun P PG c1 c2 => forall k, preord_res (preord_val cenv) PG k c1 c2) n.
+Definition pr_trivial {A} : @post_property A := fun _ _ _ _ => True.
+
+Definition wf_trivial {A} : A -> Prop := fun _ => True.
+
+
+Section RelComp.
+
+  Context (cenv : ctor_env) (ctag : ctor_tag).
+
+  Context (wf_exp : exp * env -> Prop) (post_prop : @post_property (exp * env)).
+   
+  Definition preord_exp_n n := R_n wf_exp post_prop (fun P PG c1 c2 => forall k, preord_exp cenv P PG k c1 c2) n.  
+
+  Definition preord_env_n n S := R_n wf_trivial pr_trivial (fun P PG c1 c2 => forall k, preord_env_P cenv P S k c1 c2) n.  
+
+  Definition preord_val_n n := R_n wf_trivial pr_trivial (fun P PG c1 c2 => forall k, preord_val cenv PG k c1 c2) n.
+
+  Definition preord_res_n n := R_n wf_trivial pr_trivial (fun P PG c1 c2 => forall k, preord_res (preord_val cenv) PG k c1 c2) n.
 
   Definition R_true : PostT := fun _ _ => True. 
 
@@ -43,13 +68,6 @@ Section RelComp.
   Proof.
     firstorder.
   Qed.
-
-  
-  (* Lemma preord_res_R_inn n P P' PG v : (* we just don't care *)  *)
-  (*   preord_res_n n R PG (Res v) OOT -> *)
-  (*   ~ preord_res_n n R' PG (Res v) OOT. *)
-      
-
 
   Lemma preord_res_n_OOT_r n P PG v :
     ~ preord_res_n n P PG (Res v) OOT.
@@ -90,22 +108,25 @@ Section RelComp.
       edestruct (H (k + cin)); [| eassumption | ]. omega. destructAll.
       destruct v1.
       * destruct x; eauto.
-      * destruct x; eauto. destruct x1; eauto. simpl in H6. contradiction. 
-        eapply bstep_fuel_deterministic in H1; [| clear H1; eassumption ].
-        inv H1. eapply preord_res_monotonic. eassumption. omega. 
+      * destruct x; eauto. destruct x1. contradiction.
+        eapply bstep_fuel_deterministic in H2; [| clear H2; eassumption ].
+        inv H2. eapply preord_res_monotonic. eassumption. omega.
+      * clear. firstorder.
     + destruct c1 as [e1 rho1]; destruct c2 as [e2 rho2]; destruct c' as [e' rho'].
       intros. edestruct H; eauto. destructAll.
       edestruct IHHrel. eassumption. destructAll. 
       do 2 eexists. split; eauto. split.
-      eapply H0. do 2 eexists. eassumption. eassumption. 
-      eapply More; [| eassumption | eapply R_true_idempotent | eassumption ].
+      eapply H2. do 2 eexists. eassumption. eassumption. 
+      eapply More; [| eassumption | | | eapply R_true_idempotent | eassumption ].
       destruct v1.
       * destruct x; eauto.
-      * destruct x; eauto. destruct x1. simpl in H8; eauto. simpl in H8. eapply preord_res_n_OOT_r in H8. contradiction.
+      * destruct x; eauto. destruct x1. eapply preord_res_n_OOT_r in H10. contradiction.
         intros k.
         edestruct (H (k + cin)); [| eassumption | ]. omega. destructAll. destruct x; eauto. simpl in H11. contradiction. 
-        eapply bstep_fuel_deterministic in H3; [| clear H3; eassumption ]. destructAll.
+        eapply bstep_fuel_deterministic in H5; [| clear H5; eassumption ]. destructAll.
         eapply preord_res_monotonic. eassumption. omega.
+      * clear. firstorder.
+      * clear. firstorder.        
   Qed.
   
 
@@ -118,7 +139,7 @@ Section RelComp.
     
   (* preord_exp_n preserves divergence *)
   Lemma preord_exp_n_preserves_divergence n K M P PG e1 rho1 e2 rho2 :
-    P_implies_u_bound K M (e1, rho1) (e2, rho2) P ->
+    (P_implies_u_bound K M) (e1, rho1) (e2, rho2) P ->
     preord_exp_n n P PG (e1, rho1) (e2, rho2) ->
     diverge cenv rho1 e1 -> 
     diverge cenv rho2 e2.
@@ -152,80 +173,85 @@ Section RelComp.
   Qed.
   
 
-  Definition post_propetry {A} := A -> A -> PostT -> Prop.
-
-  Definition compose_rel {A} (Pr1 Pr2 : post_propetry) (* impose things on the intermediate rels *)
-             (R1 R2 : rel) (P : PostT) (PG : PostGT) (c1 : A) (c2: A) : Prop :=
-    exists P1 P2 PG1 PG2 c',
+  Definition compose_rel {A} (P1 P2 : PostT) (PG1 PG2 : PostGT)
+             (Pr1 Pr2 : post_property) (wf : A -> Prop)
+             (R1 R2 : rel) (c1 : A) (c2: A) : Prop :=
+    exists c',
       R1 P1 PG1 c1 c' /\
       R2 P2 PG2 c' c2 /\
-      same_relation _ (compose P1 P2) P /\
-      same_relation _ (compose PG1 PG2) PG /\
-      Pr1 c1 c' P1 /\ Pr2 c' c2 P2.
+      Pr1 c1 c' P1 PG1 /\ Pr2 c' c2 P2 PG2 /\
+      wf_pres wf c1 c'.
 
-  Definition Pr_trivial {A} : @post_propetry A:= fun _ _ _ => True.
   
   (* Top-level relation for L6 pipeline *)
-  Definition R_n_exp Pr1 Pr2 Pr3 Pr4 n m : rel :=
-    compose_rel Pr1 Pr2
+  Definition R_n_exp P1 P2 P3 PG1 PG2 PG3 Pr1 Pr2 Pr3 Pr4 wf n m : relation (exp * env) :=
+    compose_rel P1 P2 PG1 PG2 Pr1 Pr2 wf
                 (preord_exp_n n)
-                (compose_rel Pr3 Pr4
-                             (fun P PG c1 c2 => forall k, cc_approx_exp cenv ctag k P PG c1 c2) (preord_exp_n m)).
+                (fun P2 PG2 => compose_rel P2 P3 PG2 PG3 Pr3 Pr4 wf
+                                           (fun P PG c1 c2 => forall k, cc_approx_exp cenv ctag k P PG c1 c2) (preord_exp_n m)).
+
+  Definition post_trivial : PostT := fun c1 c2 => True.
   
-  Definition R_n_res n m : rel :=
-    compose_rel Pr_trivial Pr_trivial (preord_res_n n)
-                (compose_rel Pr_trivial Pr_trivial (fun P PG c1 c2 => forall k, cc_approx_res (cc_approx_val cenv ctag) k PG c1 c2) (preord_res_n m)).
+  Definition R_n_res PG1 PG2 PG3 n m : relation res :=
+    compose_rel post_trivial post_trivial PG1 PG2 pr_trivial pr_trivial wf_trivial (preord_res_n n)
+                (fun P2 PG2 => compose_rel P2 post_trivial PG2 PG3 pr_trivial pr_trivial wf_trivial
+                             (fun P PG c1 c2 => forall k, cc_approx_res (cc_approx_val cenv ctag) k PG c1 c2) (preord_res_n m)).
   
-  Definition R_n_val n m : rel :=
-    compose_rel Pr_trivial Pr_trivial (preord_res_n n)
-                (compose_rel Pr_trivial Pr_trivial (fun P PG c1 c2 => forall k, cc_approx_res (cc_approx_val cenv ctag) k PG c1 c2) (preord_res_n m)).
+  Definition R_n_val PG1 PG2 PG3 n m : relation val :=
+    compose_rel post_trivial post_trivial PG1 PG2 pr_trivial pr_trivial wf_trivial (preord_val_n n)
+                (fun P2 PG2 => compose_rel P2 post_trivial PG2 PG3 pr_trivial pr_trivial wf_trivial
+                                           (fun P PG c1 c2 => forall k, cc_approx_val cenv ctag k PG c1 c2) (preord_val_n m)).
   
+
+  Definition Pr_in_P_implies_u_bound K M (Pr1 : @post_property (exp * env)) :=
+    forall p1 p2 P PG,
+      Pr1 p1 p2 P PG -> P_implies_u_bound K M p1 p2 P. 
   
-  Lemma R_n_exp_impl K M (n m : nat) (P : PostT) (PG : PostGT) e1 rho1 e2 rho2 :    
-    R_n_exp (P_implies_u_bound K M) Pr_trivial Pr_trivial Pr_trivial n m P PG (e1, rho1) (e2, rho2) ->
+  Lemma R_n_exp_impl K M P1 P2 P3 PG1 PG2 PG3 Pr1 Pr2 Pr3 Pr4 wf (n m : nat) e1 rho1 e2 rho2 :
+    Pr_in_P_implies_u_bound K M Pr1 ->
+    R_n_exp P1 P2 P3 PG1 PG2 PG3 Pr1 Pr2 Pr3 Pr4 wf n m (e1, rho1) (e2, rho2) ->    
     (forall (v1 : res) (cin : nat),
         bstep_fuel cenv rho1 e1 v1 cin ->
         not_stuck cenv rho1 e1 ->
         exists (v2 : res) (cin' : nat),
           bstep_fuel cenv rho2 e2 v2 cin' /\
-          P (e1, rho1, cin) (e2, rho2, cin') /\
-          R_n_res n m R_true PG v1 v2).
+          (comp P1 (comp P2 P3)) (e1, rho1, cin) (e2, rho2, cin') /\
+          R_n_res PG1 PG2 PG3 n m v1 v2).
   Proof.
-    intros Hrel. inv Hrel. destructAll. inv H0. destructAll.
-    assert (Hexp1 := H). assert (Hexp2 := H5).
-    eapply preord_exp_n_impl in H. 
-    eapply preord_exp_n_impl in H5.
-    destruct x3, x8. intros. edestruct H. eassumption. destructAll.    
-    edestruct (H0 x8); eauto.
-
-    eapply preord_exp_n_preserves_not_stuck; eassumption.
+    intros Himpl Hrel. inv Hrel. destructAll. inv H0. destructAll. 
+    assert (Hexp1 := H). assert (Hexp2 := H4).
+    eapply preord_exp_n_impl in H.  
+    eapply preord_exp_n_impl in H4.
+    destruct x, x0. intros. edestruct H. eassumption. destructAll.    
+    edestruct (H0 x0); eauto.
     
-    destructAll. edestruct H5. eassumption. destructAll.
+    eapply preord_exp_n_preserves_not_stuck. eapply Himpl. eassumption. eassumption. eassumption.
+    
+    destructAll. edestruct H4. eassumption. destructAll.
     
     do 2 eexists. split; eauto. split; eauto.
 
-    eapply H1. eexists. split. eassumption. eapply H6. eexists. split; eassumption.
+    eexists. split. eassumption. eexists. split; eassumption.
 
-    do 5 eexists. split. eassumption.
-    split; [| split; [ now eapply R_true_idempotent |  split; [ eassumption | now clear; firstorder ]]]. 
-
-    do 5 eexists. split; [| split; [| split; [ now eapply R_true_idempotent | split; [ eassumption | now clear; firstorder ]]]].
-    2:{ eassumption. }
-
+    eexists. split. eassumption. split.
+    2:{ split. clear. now firstorder. split. now firstorder. now firstorder. }
+    eexists. split.
+    2:{ split. eassumption. split. now firstorder. now firstorder. }
+    
     intros k. 
     destruct v1.
-    - destruct x3.
-      * destruct x9; eauto.
-      * eapply preord_res_n_OOT_l in H14. contradiction.
-    - destruct x3.
-      + eapply preord_res_n_OOT_r in H14. contradiction.
-      + destruct x9; eauto.
-        edestruct (H0 (k + x8)); [| eassumption | | ]. omega.
-        eapply preord_exp_n_preserves_not_stuck; eassumption.
-
+    - destruct x.
+      * destruct x1; eauto. 
+      * eapply preord_res_n_OOT_l in H12. contradiction.
+    - destruct x.
+      + eapply preord_res_n_OOT_r in H12. contradiction.
+      + destruct x1; eauto.
+        edestruct (H0 (k + x0)); [| eassumption | | ]. omega.
+        eapply preord_exp_n_preserves_not_stuck. eapply Himpl. eassumption. eassumption. eassumption.
+        
         destructAll.
-        destruct x3. simpl in H18. contradiction.
-        eapply bstep_fuel_deterministic in H15; [| clear H15; eassumption ]. inv H15.
+        destruct x. contradiction.
+        eapply bstep_fuel_deterministic in H19; [| clear H19; eassumption ]. inv H19.
         eapply cc_approx_res_monotonic. eassumption. omega.
   Qed.
 
@@ -249,78 +275,449 @@ Section RelComp.
     + eapply bstep_fuel_OOT_monotonic. eassumption. eassumption.
     + contradiction.
   Qed.
-
+  
   
   (* R_n_exp preserves divergence *)
-  Lemma R_n_exp_preserves_divergence n m K1 M1 K2 M2 K3 M3 P PG e1 rho1 e2 rho2 :
-    R_n_exp (P_implies_u_bound K1 M1) Pr_trivial (P_implies_u_bound K2 M2) (P_implies_u_bound K3 M3) n m P PG (e1, rho1) (e2, rho2) ->
+  Lemma R_n_exp_preserves_divergence n m K1 M1 K2 M2 K3 M3 P1 P2 P3 PG1 PG2 PG3 Pr1 Pr2 Pr3 Pr4 wf e1 rho1 e2 rho2 :
+    Pr_in_P_implies_u_bound K1 M1 Pr1 ->
+    Pr_in_P_implies_u_bound K2 M2 Pr3 ->
+    Pr_in_P_implies_u_bound K3 M3 Pr4 ->
+    R_n_exp P1 P2 P3 PG1 PG2 PG3 Pr1 Pr2 Pr3 Pr4 n m wf (e1, rho1) (e2, rho2) ->
     diverge cenv rho1 e1 -> 
     diverge cenv rho2 e2.
   Proof.
-    intros Hrel Hdiv. inv Hrel. destructAll. destruct x3. inv H0. destructAll. destruct x7. 
-    eapply preord_exp_n_preserves_divergence; [ eassumption | eassumption | ].
-    eapply cc_approx_exp_rreserves_divergence; [ eassumption | eassumption | ].
-    eapply preord_exp_n_preserves_divergence; eassumption.
+    intros Hp1 Hp2 Hp3 Hrel Hdiv. inv Hrel. destructAll. destruct x. inv H0. destructAll. destruct x. 
+    eapply preord_exp_n_preserves_divergence; [| eassumption | ];
+      [| eapply cc_approx_exp_rreserves_divergence; [ | eassumption | ];
+         [| eapply preord_exp_n_preserves_divergence; [| eassumption | eassumption ] ]].
+    eapply Hp3. eassumption. eapply Hp2. eassumption. eapply Hp1. eassumption.
   Qed.
 
+End RelComp.
 
+Section Linking.
   
-  Section Linking.
+  Context (lft: fun_tag).
+  Context (cenv : ctor_env) (ctag : ctor_tag).
+    
+  Definition link_src (e1 e2 : exp) : option exp :=
+    match e2 with
+    | Efun (Fcons f ft [x] e Fnil) (Ehalt f') =>
+      if (f =? f')%positive && (ft =? lft)%positive  then  
+        match inline_letapp e1 x with
+        | Some (C, x') =>
+          if (x' =? f')%positive then None (* shadowing happens *)                                          
+          else Some (C |[ Efun (Fcons f lft [x] e Fnil) (Eapp f lft [x'])]|)
+        | None => None
+        end
+      else None
+    | _ => None
+    end.
 
-    Definition link_src (e1 e2 : exp) : option exp :=
-      match e2 with
-      | Efun (Fcons f ft [x] e Fnil) (Ehalt f') =>
-        if (f =? f')%positive then  
-          match inline_letapp e x with
-          | Some (C, x') =>
-            Some (C |[ Efun (Fcons f ft [x] e Fnil) (Eapp f ft [x'])]|)
-          | None => None
-          end
-        else None
-      | _ => None
-      end.
-
-    Definition link_trg (e1 e2 : exp) : option exp :=
-      match e2 with
-      | Efun (Fcons f ft [x] e Fnil) (Ehalt f') =>
-        if (f =? f')%positive then  
-          match inline_letapp e x with
-          | Some (C, x') =>
+  Definition link_trg (e1 e2 : exp) : option exp :=
+    match e2 with
+    | Efun (Fcons f ft [x] e Fnil) (Ehalt f') =>
+      if (f =? f')%positive && (ft =? lft)%positive then  
+        match inline_letapp e1 x with
+        | Some (C, x') =>
+          if (x' =? f')%positive then None (* shadowing happens *)
+          else
             let fv := max_var e1 f in
             let f' := (fv + 1)%positive in
             let Γ := (fv + 2)%positive in
-            Some (C |[ Efun (Fcons f ft [x] e Fnil) (AppClo ctag f f' Γ |[ Eapp f ft [Γ; x] ]|) ]|)
-          | None => None
-          end
-        else None
-      | _ => None
-      end.
+            Some (C |[ Efun (Fcons f lft [x] e Fnil) (AppClo ctag f f' Γ |[ Eapp f lft [Γ; x] ]|) ]|)
+        | None => None
+        end
+      else None
+    | _ => None
+    end.
 
 
-    Lemma preord_exp_preserves_linking_src k P PG e1 e2 e1' e2' :
-      preord_exp cenv P PG k (e1, M.empty _) (e2, M.empty _) ->
-      preord_exp cenv P PG k (e1', M.empty _) (e2', M.empty _) ->
-      match link_src e1 e1', link_src e2 e2' with
-      | Some e, Some e' =>
-        preord_exp cenv P PG k (e, M.empty _) (e', M.empty _)
-      | _ , _ => True
-      end.
+  Definition rel_union {A} (P1 P2 : relation A) :=
+    fun c1 c2 => P1 c1 c2 \/ P2 c1 c2.
+  
+  Definition id_rel {A} : relation A := fun x y => x = y.
+
+  
+  Lemma id_rel_neut_l {A} P :
+    same_relation A (compose P id_rel) P.
+  Proof.
+    split; intro; intros.
+    + unfold compose, id_rel in H. destructAll. eassumption.
+    + unfold compose, id_rel. eexists; split; eauto.
+  Qed.
+
+  Lemma id_rel_neut_r {A} P :
+    same_relation A (compose id_rel P) P.
+  Proof.
+    split; intro; intros.
+    + unfold compose, id_rel in H. destructAll. eassumption.
+    + unfold compose, id_rel. eexists; split; eauto.
+  Qed.
+
+    
+  Context (P : PostT) (PG : PostGT)
+          (Hinl : post_inline cenv P P P)
+          (HinlOOT : post_inline_OOT P P)
+          (Hpost : post_fun_compat P P)
+          (HpostOOT : post_OOT P)
+          (Hpostapp: post_app_compat P PG).
+
+  
+  Lemma preord_exp_preserves_linking_src k e1 e2 e1' e2' :
+    
+    (forall k rho1 rho2,
+        preord_exp cenv P PG k (e1, rho1) (e2, rho2)) ->
+    
+    (forall k rho1 rho2,
+        preord_exp cenv P PG k (e1', rho1) (e2', rho2)) ->
+    
+    closed_exp e1 ->
+    closed_exp e1' ->
+    
+    match link_src e1 e1', link_src e2 e2' with
+    | Some e, Some e' =>
+      preord_exp cenv P PG k (e, M.empty _) (e', M.empty _)
+    | _ , _ => True
+    end.
+  Proof.
+    intros Hexp1 Hexp2 Hc1 Hc2. unfold link_src.
+    
+    destruct e1'; eauto. destruct f; eauto. destruct l; eauto. destruct l; eauto.
+    destruct f0; eauto.  destruct e1'; eauto.
+    destruct ((v =? v1)%positive && (f =? lft)%positive) eqn:Hfeq; eauto.
+    destruct (inline_letapp e1 v0) as [[C z] | ] eqn:Hinl1; eauto.
+    destruct ((z =? v1)%positive) eqn:Hs; eauto.      
+    
+    destruct e2'; eauto. destruct f0; eauto. destruct l; eauto. destruct l; eauto.
+    destruct f1; eauto.  destruct e2'; eauto.
+    destruct ((v2 =? v4)%positive && (f0 =? lft)%positive) eqn:Hfeq'; eauto.
+    destruct (inline_letapp e2 v3) as [[C' z'] | ] eqn:Hinl2; eauto.
+    destruct ((z' =? v4)%positive) eqn:Hs'; eauto.
+    
+    eapply andb_prop in Hfeq. eapply andb_prop in Hfeq'. destructAll. 
+    eapply Peqb_true_eq in H1. eapply Peqb_true_eq in H2.
+    eapply Peqb_true_eq in H. eapply Peqb_true_eq in H0. subst.
+    eapply Pos.eqb_neq in Hs. eapply Pos.eqb_neq in Hs'.
+    
+    eapply inline_letapp_compat with (sig := id); [ | | | eapply Hc1 | eassumption | eassumption  | | ].
+    - eassumption.
+    - eassumption.
+    - intros. eapply Hexp1.
+    - intros. eapply preord_exp_fun_compat.
+      + eassumption.
+      + eassumption.
+      + assert (Hvalrel :
+                  forall k,
+                    preord_env_P cenv PG (Empty_set _) k rho1 rho2 ->
+                    preord_val cenv PG k (Vfun rho1 (Fcons v1 lft [v0] e Fnil) v1) (Vfun rho2 (Fcons v4 lft [v3] e0 Fnil) v4)).
+        { intros j. edestruct (Hexp2 (j + 2) rho1 rho2) with (cin:= 2).
+          
+          omega.
+          
+          econstructor 2. simpl. omega.
+          simpl. econstructor. simpl. econstructor 2. simpl. omega.  econstructor.
+          rewrite M.gss. reflexivity.
+          destructAll. inv H1. contradiction. inv H5. inv H10. contradiction. inv H5.
+          simpl in H10. rewrite M.gss in H10. inv H10.
+          simpl in H3. 
+          simpl. intros Henv. eapply preord_val_monotonic. 
+          eassumption. omega. }
+        
+          simpl. eapply preord_exp_app_compat.
+        * eassumption.
+        * eassumption.
+        * simpl. intros w Hget. rewrite M.gss in Hget. inv Hget. 
+          eexists. rewrite M.gss. split. reflexivity. eapply Hvalrel.
+          intros x Hin. inv Hin.
+        * constructor; [| now constructor ].
+          
+          simpl. intros w1 Hget.
+          rewrite M.gso in Hget; auto. 
+          rewrite M.gso; auto.
+          eapply H0 in Hget; [| reflexivity ]. destructAll.
+          rewrite functions.extend_gss in H1. 
+          eexists. split; eauto. eapply preord_val_monotonic. eassumption. omega. 
+    - intros x Hin v Hget. rewrite M.gempty in Hget. inv Hget.
+  Qed.
+
+
+    Class Post_properties (P1 : PostT) (PG : PostGT) : Prop :=
+    { HPost_con : post_constr_compat P1 P1;
+      HPost_proj : post_proj_compat P1 P1;
+      HPost_fun : post_fun_compat P1 P1;
+      HPost_case_hd : post_case_compat_hd P1 P1;
+      HPost_case_tl : post_case_compat_tl P1 P1;
+      HPost_app : post_app_compat P1 PG;
+      HPost_letapp : post_letapp_compat cenv P1 P1 PG;
+      HPost_letapp_OOT : post_letapp_compat_OOT P1 PG;
+      HPost_OOT : post_OOT P1;
+      Hpost_base : post_base P1;
+      HGPost : inclusion _ P1 PG }.
+
+    Definition Post_id : PostT := fun c1 c2 => c1 = c2.
+
+    Lemma preord_exp_refl k e rho rho' :
+    preord_env_P cenv Post_id (occurs_free e) k rho rho' ->
+    preord_exp cenv Post_id Post_id k (e, rho) (e, rho').
+  Proof with eauto with Ensembles_DB.
+    revert e rho rho'.
+    (* Well founded induction on the step-index *)
+    induction k as [ k IH ] using lt_wf_rec1.
+    (* Induction on e *) 
+    intros e. revert k IH.
+    induction e using exp_ind'; intros k IH rho rho' Henv. 
+    (* Each case follows from the corresponding compat lemma *)
+    - eapply preord_exp_const_compat with (P1 := Post_id); eauto; intros.
+      * clear. intro; intros. intro; intros. unfold Post_id in *.
+        inv H1. firstorder. eapply Forall2_same. intros x HIn. apply Henv. now constructor.
+      * eapply IHe. intros. eapply IH; eauto. omega.
+        eapply preord_env_P_extend.
+        eapply preord_env_P_antimon. eapply preord_env_P_monotonic; [| eassumption ].
+        omega.
+        now (normalize_occurs_free; eauto with Ensembles_DB). 
+        rewrite preord_val_eq. constructor; eauto using Forall2_Forall2_asym_included.
+    - eapply preord_exp_case_nil_compat. eassumption.
+    - eapply preord_exp_case_cons_compat; eauto.
+      now apply Forall2_refl.
+      intros m Hlt. apply IHe; try eassumption.
+      intros. eapply IH; eauto. omega.
+      eapply preord_env_P_antimon. 
+      eapply preord_env_P_monotonic; [| eassumption ]. omega.
+      normalize_occurs_free. sets.
+      eapply IHe0; eauto.
+      eapply preord_env_P_antimon. 
+      eapply preord_env_P_monotonic; [| eassumption ]. omega.
+      normalize_occurs_free. sets.
+    - eapply preord_exp_proj_compat; eauto.
+      intros m v1 v2 Hlt Hval. apply IHe; try eassumption.
+      intros. eapply IH; eauto. omega.
+      eapply preord_env_P_extend; eauto.
+      eapply preord_env_P_antimon.
+      eapply preord_env_P_monotonic; [| eassumption ]. omega.
+      now (normalize_occurs_free; eauto with Ensembles_DB).
+    - eapply preord_exp_letapp_compat; eauto.
+      eapply Henv. constructor. now left.
+      eapply Forall2_same. intros. apply Henv. constructor. now right.
+      intros m v1 v2 Hlt Hval. 
+      eapply IHe; try eassumption.
+      intros. eapply IH; eauto. omega.
+      eapply preord_env_P_extend; eauto.
+      eapply preord_env_P_antimon.
+      eapply preord_env_P_monotonic; [| eassumption ]. omega.
+      now (normalize_occurs_free; eauto with Ensembles_DB).
+    - eapply preord_exp_fun_compat; eauto.
+      eapply IHe; try eassumption. 
+      intros. eapply IH; eauto. omega. 
+      eapply preord_env_P_antimon.
+      eapply preord_env_P_def_funs_pre; eauto.
+      intros. eapply IH; eauto. omega. 
+      eapply preord_env_P_monotonic; [| eassumption ]. omega.
+      now eapply occurs_free_Efun_Included.
+    - eapply preord_exp_app_compat. eassumption. eassumption.
+      intros x HP. apply Henv; eauto.
+      apply Forall2_same. intros. apply Henv. now constructor.
+    - eapply preord_exp_prim_compat; eauto; intros.
+      eapply Forall2_same. intros. apply Henv. now constructor.
+    - eapply preord_exp_halt_compat; try eassumption.
+      intros x HP. apply Henv; eauto.
+   Qed.
+
+    Instance Post_properties_post_id : Post_properties Post_id Post_id.
     Proof.
-      intros Hexp1 Hexp2. unfold link_src.
-      
-      destruct e1'; eauto. destruct f; eauto. destruct l; eauto. destruct l; eauto.
-      destruct f0; eauto.  destruct e1'; eauto. destruct ((v =? v1)%positive); eauto.
-      destruct (inline_letapp e v0) as [[C z] | ] eqn:Hinl1; eauto.
+      constructor.
+      - intro; intros. intro; intros. unfold Post_id in *. simpl in *. inv H1.
+        reflexivity. 
+      - intro; intros. intro; intros. unfold Post_id in *. simpl in *. inv H1.
+        reflexivity. 
+      - intro; intros. intro; intros. unfold Post_id in *. simpl in *. subst.
+        reflexivity.
+      - intro; intros. intro; intros. unfold Post_id in *. simpl in *. subst.
+        reflexivity. 
+      - intro; intros. intro; intros. unfold Post_id in *. simpl in *. subst.
+        reflexivity.
+      - intro; intros. intro; intros. unfold Post_id in *. simpl in *. inv H1.
+        reflexivity. 
+      - intro; intros. intro; intros. unfold Post_id in *. simpl in *. subst. reflexivity.
+      - intro; intros. intro; intros. unfold Post_id in *. simpl in *. subst. reflexivity.
+      - intro; intros. intro; intros. unfold Post_id in *. simpl in *. subst. reflexivity.
+      - intro; intros. intro; intros. unfold Post_id in *. simpl in *. subst. reflexivity.
+      - firstorder.
+    Qed. 
+    
+    Context (P1 P2 : PostT) (PG1 PG2 : PostGT).
 
-      destruct e2'; eauto. destruct f0; eauto. destruct l; eauto. destruct l; eauto.
-      destruct f1; eauto.  destruct e2'; eauto. destruct ((v2 =? v4)%positive); eauto.
-      destruct (inline_letapp e0 v3) as [[C' z'] | ] eqn:Hinl2; eauto.
-      
-      
-      
+
+  Definition closed_conf (c : exp * env) := closed_exp (fst c).
+
+
+  Lemma preord_exp_n_0 k Pr e1 rho1 e2 rho2 :
+    preord_exp_n cenv closed_conf Pr 0 P1 PG1 (e1, rho1) (e2, rho2) ->
+    preord_exp cenv P1 PG1 k (e1, rho1) (e2, rho2).
+  Proof.
+    intros H. inv H. eauto.
+  Qed.
 
       
-      ; destruct e2'; eauto. 
-      destruct e1. 
+  Context (HPost_con : post_constr_compat P1 P1)
+          (HPost_proj : post_proj_compat P1 P1)
+          (HPost_fun : post_fun_compat P1 P1)
+          (HPost_case_hd : post_case_compat_hd P1 P1)
+          (HPost_case_tl : post_case_compat_tl P1 P1)
+          (HPost_app : post_app_compat P1 PG1)
+          (HPost_letapp : post_letapp_compat cenv P1 P1 PG1)
+          (HPost_letapp_OOT : post_letapp_compat_OOT P1 PG1)
+          (HPost_OOT : post_OOT P1)
+          (Hpost_base : post_base P1)
+          (HGPost : inclusion _ P1 PG1)
+          (HPost_conG : post_constr_compat PG1 PG1)
+          (HPost_projG : post_proj_compat PG1 PG1)
+          (HPost_funG : post_fun_compat PG1 PG1)
+          (HPost_case_hdG : post_case_compat_hd PG1 PG1)
+          (HPost_case_tlG : post_case_compat_tl PG1 PG1)
+          (HPost_appG : post_app_compat PG1 PG1)
+          (HPost_letappG : post_letapp_compat cenv PG1 PG1 PG1)
+          (HPost_letapp_OOTG : post_letapp_compat_OOT PG1 PG1)
+          (HPost_OOTG : post_OOT PG1)
+          (Hpost_baseG : post_base PG1).
+  
+    
+  
+  Lemma preord_exp_n_refl n Pr e1 rho1 :
+    preord_exp_n cenv closed_conf Pr n P1 PG1 (e1, rho1) (e1, rho1).
+  Proof.
+    induction n.
+    - constructor; [| clear; firstorder ].
+      intros k. eapply preord_exp_refl; eauto. 
+      eapply preord_env_P_refl; eauto.
+    - econstructor.       
+      2:{ eapply 
+      + intros 
+      intros H. inv H. eauto.
+  Qed.
+
+  Lemma preord_exp_n_m n m Pr e1 rho1 e2 rho2 :
+    preord_exp_n cenv closed_conf Pr n P1 PG1 (e1, rho1) (e2, rho2) ->
+    n <= m ->
+    preord_exp_n cenv closed_conf Pr m P1 PG1 (e1, rho1) (e2, rho2).
+  Proof.
+    revert n Pr e1 rho1 e2 rho2. induction m using lt_wf_rec1; intros n Pr e1 rho1 e2 rho2 Hexp Hlt.
+    destruct m. 
+    - destruct n. eassumption. omega.
+    - econstructor. intros k. eapply preord_exp_refl. 
+      admit.
+      admit.
+      admit.
+      admit.
+      admit.
+      admit.
+      admit.
+      admit.
+      admit.
+      admit.
+      admit.
+      eapply preord_env_P_refl.
+      admit.
+      admit.
+      admit.
+      admit.
+      admit.
+      admit.
+      admit.
+      admit.
+      admit.
+      admit.
+      eapply H. omega. eassumption. omega. admit.
       
+      admit.
       
+    intros H. inv H. eauto.
+  Qed.
+
+  Lemma preord_exp_n_preserves_linking_src n e1 e2 e1' e2' Pr :
+    
+    (forall rho1 rho2,
+        preord_exp_n cenv closed_conf Pr n P1 PG1 (e1, rho1) (e2, rho2)) ->
+    
+    (forall rho1 rho2,
+        preord_exp_n cenv closed_conf Pr n P2 PG2 (e1', rho1) (e2', rho2)) ->
+    
+    closed_exp e1 ->
+    closed_exp e1' ->
+    
+    match link_src e1 e1', link_src e2 e2' with
+    | Some e, Some e' =>
+      preord_exp_n cenv closed_conf Pr n (comp P1 P2) (comp PG1 PG2) (e, M.empty _) (e', M.empty _)
+    | _ , _ => True
+    end.
+  Proof.
+    revert e1 e2 e1' e2' Pr. induction n; intros e1 e2 e1' e2' Pr.
+    + intros Hexp1 Hexp2 Hc1 Hc2. unfold link_src.
+    
+    destruct e1'; eauto. destruct f; eauto. destruct l; eauto. destruct l; eauto.
+    destruct f0; eauto.  destruct e1'; eauto.
+    destruct ((v =? v1)%positive && (f =? lft)%positive) eqn:Hfeq; eauto.
+    destruct (inline_letapp e1 v0) as [[C z] | ] eqn:Hinl1; eauto.
+    destruct ((z =? v1)%positive) eqn:Hs; eauto.      
+    
+    destruct e2'; eauto. destruct f0; eauto. destruct l; eauto. destruct l; eauto.
+    destruct f1; eauto.  destruct e2'; eauto.
+    destruct ((v2 =? v4)%positive && (f0 =? lft)%positive) eqn:Hfeq'; eauto.
+    destruct (inline_letapp e2 v3) as [[C' z'] | ] eqn:Hinl2; eauto.
+    destruct ((z' =? v4)%positive) eqn:Hs'; eauto.
+    
+    eapply andb_prop in Hfeq. eapply andb_prop in Hfeq'. destructAll. 
+    eapply Peqb_true_eq in H1. eapply Peqb_true_eq in H2.
+    eapply Peqb_true_eq in H. eapply Peqb_true_eq in H0. subst.
+    eapply Pos.eqb_neq in Hs. eapply Pos.eqb_neq in Hs'.
+
+    revert e1 e2 e1' e2' Pr
+    eapply inline_letapp_compat with (sig := id); [ | | | eapply Hc1 | eassumption | eassumption  | | ].
+    - eassumption.
+    - eassumption.
+    - intros. eapply Hexp1. eapply preord_env_P_antimon; [| eapply Hc1 ].
+      intros x Hin. inv Hin.
+    - intros. eapply preord_exp_fun_compat.
+      + eassumption.
+      + eassumption.
+      + assert (Hvalrel :
+                  forall k,
+                    preord_env_P cenv PG (Empty_set _) k rho1 rho2 ->
+                    preord_val cenv PG k (Vfun rho1 (Fcons v1 lft [v0] e Fnil) v1) (Vfun rho2 (Fcons v4 lft [v3] e0 Fnil) v4)).
+        { intros j. edestruct (Hexp2 (j + 2) rho1 rho2) with (cin:= 2).
+          
+          eapply preord_env_P_antimon; [| eapply Hc2 ].
+            intros x Hin. now inv Hin.      
+            
+            omega.
+            
+            econstructor 2. simpl. omega.
+            simpl. econstructor. simpl. econstructor 2. simpl. omega.  econstructor.
+            rewrite M.gss. reflexivity.
+            destructAll. inv H1. contradiction. inv H5. inv H10. contradiction. inv H5.
+            simpl in H10. rewrite M.gss in H10. inv H10.
+            simpl in H3. 
+            simpl. intros Henv. eapply preord_val_monotonic. 
+            eassumption. omega. }
+          
+          simpl. eapply preord_exp_app_compat.
+        * eassumption.
+        * eassumption.
+        * simpl. intros w Hget. rewrite M.gss in Hget. inv Hget. 
+          eexists. rewrite M.gss. split. reflexivity. eapply Hvalrel.
+          intros x Hin. inv Hin.
+        * constructor; [| now constructor ].
+          
+          simpl. intros w1 Hget.
+          rewrite M.gso in Hget; auto. 
+          rewrite M.gso; auto.
+          eapply H0 in Hget; [| reflexivity ]. destructAll.
+          rewrite functions.extend_gss in H1. 
+          eexists. split; eauto. eapply preord_val_monotonic. eassumption. omega. 
+    - intros x Hin v Hget. rewrite M.gempty in Hget. inv Hget.
+  Qed.        
+
+
+  End Linking.
+
+End RelComp.
